> [!Example]-
> $$
> \displaylines{
> 	\mathbf{Y} \times \mathbf{Z}
> 	=\\\\
> 	\begin{bmatrix}
> 		0 & -i\\
> 		i & 0
> 	\end{bmatrix}
> 	\times
> 	\begin{bmatrix}
> 		1 & 0\\
> 		0 & -1
> 	\end{bmatrix}
> 	=\\\\
> 	\begin{bmatrix}
> 		(0 \cdot 1) + (-i \cdot 0) & (0 \cdot 0) + (-i \cdot -1)\\
> 		(i \cdot 1) + (0 \cdot 0) & (i \cdot 0) + (-1 \cdot 0)
> 	\end{bmatrix}
> 	=\\\\
> 	\begin{bmatrix}
> 		0 & i\\
> 		i & 0
> 	\end{bmatrix}
> 	=\\\\
> 	i \cdot
> 	\begin{bmatrix}
> 		0 & 1\\
> 		1 & 0
> 	\end{bmatrix}
> 	=\\\\
> 	i \cdot \mathbf{X}
> }
> $$

